Hom work

Kura/Operation/Hom.lean
@@ -1,9 +1,9 @@
-import Kura.Graph
+import Kura.Isolated
 
 
 open Set Function
-variable {α β α' β' γ δ ε ζ : Type*} {G₁ : Graph α β} {G₂ : Graph γ δ} {G₃ : Graph ε ζ} {a b c : α}
-  {e f : β} {u v w : γ} {x y z : δ}
+variable {α β α' β' γ δ ε ζ : Type*} {G G₁ : Graph α β} {G₂ : Graph γ δ} {G₃ : Graph ε ζ}
+  {a b c : α} {e f : β} {u v w : γ} {x y z : δ} {S S' T T' U U': Set α} {F F' R R' : Set β}
 namespace Graph
 
 
@@ -21,52 +21,112 @@ instance : CoeFun (HomSys α β α' β') fun (_ : HomSys α β α' β') ↦ α �
 -- structure HomSys.IsLawful (G : Graph α β) (f : HomSys α β γ δ) : Prop where
 --   forall_foo : ∀ e x y, G.Inc₂ e x y →
 
-def map (G : Graph α β) (f : HomSys α β α' β') : Graph α' β' where
-  V := f '' G.V
-  E := f.edgeFun '' G.E
-  Inc x e := ∃ x₀ e₀, G.Inc x₀ e₀ ∧ x = f x₀ ∧ e = f.edgeFun e₀
-  vx_mem_of_inc := sorry
-  edge_mem_of_inc := sorry
-  exists_vertex_inc := sorry
-  not_hypergraph := sorry
-
 -- instance : CoeFun (HomSys α β γ δ) fun (_ : HomSys α β γ δ) ↦ β → δ where
 --   coe v := v.fₑ
 
-def HomSys.id : HomSys α β α β where
-  toFun := _root_.id
-  edgeFun := _root_.id
-
-def HomSys.comp (g : HomSys α β γ δ) (f : HomSys γ δ ε ζ) : HomSys α β ε ζ where
-  toFun := f ∘ g
-  edgeFun := f.edgeFun ∘ g.edgeFun
-
-def HomSys.IsHomOn (f : HomSys α β γ δ) (G₁ : Graph α β) (G₂ : Graph γ δ) : Prop :=
-  ∀ ⦃e x y⦄, G₁.Inc₂ e x y → G₂.Inc₂ (f.edgeFun e) (f x) (f y)
+structure HomSys.IsHomOn (f : HomSys α β γ δ) (G₁ : Graph α β) (G₂ : Graph γ δ) : Prop where
+  Mapsto_vx : MapsTo f G₁.V G₂.V
+  inc₂ ⦃e x y⦄ : G₁.Inc₂ e x y → G₂.Inc₂ (f.edgeFun e) (f x) (f y)
+  Mapsto_edge : MapsTo f.edgeFun G₁.E G₂.E :=
+    fun _ he ↦ (inc₂ (Inc₂.exists_vx_inc₂ he).choose_spec.choose_spec).edge_mem
 
 def HasHom (G₁ : Graph α β) (G₂ : Graph γ δ) := ∃ f : HomSys α β γ δ, f.IsHomOn G₁ G₂
 
-def HomSys.EmbOn (f : HomSys α β γ δ) (G₁ : Graph α β) (G₂ : Graph γ δ) : Prop :=
-  f.IsHomOn G₁ G₂ ∧ InjOn f G₁.V ∧ InjOn f.edgeFun G₁.E
+scoped infix:50 " ≤⟶ " => HasHom
 
-def HasEmb (G₁ : Graph α β) (G₂ : Graph γ δ) := ∃ f : HomSys α β γ δ, f.EmbOn G₁ G₂
+structure HomSys.IsEmbOn (f : HomSys α β γ δ) (G₁ : Graph α β) (G₂ : Graph γ δ) : Prop extends
+  IsHomOn f G₁ G₂ where
+  injOn_vx : InjOn f G₁.V
+  injOn_edge : InjOn f.edgeFun G₁.E
+
+def HasEmb (G₁ : Graph α β) (G₂ : Graph γ δ) := ∃ f : HomSys α β γ δ, f.IsEmbOn G₁ G₂
+
+scoped infix:50 " ≤↪ " => HasEmb
 
 def HasEmb.toHasHom {G₁ : Graph α β} {G₂ : Graph γ δ} (h : HasEmb G₁ G₂) : HasHom G₁ G₂ := by
   obtain ⟨f, hf⟩ := h
   exact ⟨f, hf.1⟩
 
-structure HomSys.IsIsomOn (f : HomSys α β γ δ) (G₁ : Graph α β) (G₂ : Graph γ δ) : Prop where
-  isHomOn : f.IsHomOn G₁ G₂
+structure HomSys.IsIsomOn (f : HomSys α β γ δ) (G₁ : Graph α β) (G₂ : Graph γ δ) : Prop extends
+  IsHomOn f G₁ G₂ where
   bij_vertex : BijOn f G₁.V G₂.V
   bij_edge : BijOn f.edgeFun G₁.E G₂.E
 
 def HasIsom (G₁ : Graph α β) (G₂ : Graph γ δ) := ∃ f : HomSys α β γ δ, f.IsIsomOn G₁ G₂
 
+scoped infix:50 " ≤↔ " => HasIsom
+
 lemma HasIsom.toHasEmb {G₁ : Graph α β} {G₂ : Graph γ δ} (h : HasIsom G₁ G₂) : HasEmb G₁ G₂ := by
-  obtain ⟨f, hHomOn, hvinj, feinj, hvsurj, fsurj⟩ := h
-  sorry
-  -- exact ⟨f, ⟨hHomOn, hvinj, feinj⟩⟩
+  obtain ⟨f, hHomOn, ⟨fvMps, fvInj, fvSurj⟩, feMps, heInj, feSurj⟩ := h
+  use f, hHomOn
 
 lemma  HasIsom.toHasHom {G₁ : Graph α β} {G₂ : Graph γ δ} (h : HasIsom G₁ G₂) : HasHom G₁ G₂ := by
-  obtain ⟨f, hHomOn, hvinj, feinj, hvsurj, fsurj⟩ := h
+  obtain ⟨f, hHomOn, ⟨fvMps, fvInj, fvSurj⟩, feMps, heInj, feSurj⟩ := h
   exact ⟨f, hHomOn⟩
+
+def HomSys.id : HomSys α β α β where
+  toFun := _root_.id
+  edgeFun := _root_.id
+
+lemma HomSys.IsHomOn.id : HomSys.id.IsHomOn G G where
+  Mapsto_vx := fun ⦃_⦄ a ↦ a
+  inc₂ := fun ⦃_ _ _⦄ a ↦ a
+
+lemma HomSys.IsEmbOn.id : HomSys.id.IsEmbOn G G :=
+  ⟨HomSys.IsHomOn.id, injOn_id G.V, injOn_id G.E⟩
+
+lemma HomSys.IsIsomOn.id : HomSys.id.IsIsomOn G G :=
+  ⟨HomSys.IsHomOn.id, bijOn_id G.V, bijOn_id G.E⟩
+
+def HomSys.comp (g : HomSys α β γ δ) (f : HomSys γ δ ε ζ) : HomSys α β ε ζ where
+  toFun := f ∘ g
+  edgeFun := f.edgeFun ∘ g.edgeFun
+
+lemma HomSys.IsHomOn.comp {g : HomSys α β γ δ} {f : HomSys γ δ ε ζ} (hg : g.IsHomOn G₁ G₂)
+    (hf : f.IsHomOn G₂ G₃) : (g.comp f).IsHomOn G₁ G₃ where
+  Mapsto_vx := fun ⦃_⦄ a ↦ hf.Mapsto_vx (hg.Mapsto_vx a)
+  inc₂ := fun ⦃_ _ _⦄ a ↦ hf.inc₂ (hg.inc₂ a)
+
+lemma HomSys.IsEmbOn.comp {g : HomSys α β γ δ} {f : HomSys γ δ ε ζ} (hg : g.IsEmbOn G₁ G₂)
+    (hf : f.IsEmbOn G₂ G₃) : (g.comp f).IsEmbOn G₁ G₃ where
+  toIsHomOn := hg.toIsHomOn.comp hf.toIsHomOn
+  injOn_vx := hf.injOn_vx.comp hg.injOn_vx hg.Mapsto_vx
+  injOn_edge := hf.injOn_edge.comp hg.injOn_edge hg.Mapsto_edge
+
+lemma HomSys.IsIsomOn.comp {g : HomSys α β γ δ} {f : HomSys γ δ ε ζ} (hg : g.IsIsomOn G₁ G₂)
+    (hf : f.IsIsomOn G₂ G₃) : (g.comp f).IsIsomOn G₁ G₃ where
+  toIsHomOn := hg.toIsHomOn.comp hf.toIsHomOn
+  bij_vertex := hf.bij_vertex.comp hg.bij_vertex
+  bij_edge := hf.bij_edge.comp hg.bij_edge
+
+section Hom
+
+lemma HasHom.bot [hg : Nonempty γ] [hd : Nonempty δ] : (⊥ : Graph α β) ≤⟶ G₂ := by
+  use ⟨fun _ ↦ hg.some, fun _ ↦ hd.some⟩
+  exact {
+    Mapsto_vx := mapsTo_empty (fun x ↦ hg.some) G₂.V
+    inc₂ := fun e x y hbtw ↦ by
+      simp only [bot_E, mem_empty_iff_false, not_false_eq_true, not_inc₂_of_not_edge_mem] at hbtw}
+
+lemma HasHom.edgeless [hd : Nonempty δ] (hU : U.Nonempty) : (Edgeless U β) ≤⟶ G₂ ↔ G₂.V.Nonempty := by
+  constructor
+  · rintro ⟨f, hsu, hf⟩
+    use f hU.some, hsu (by simp [hU.some_mem])
+  · rintro ⟨v, hv⟩
+    use ⟨fun _ ↦ v, fun _ ↦ hd.some⟩
+    exact {
+      Mapsto_vx := fun ⦃x⦄ a ↦ hv
+      inc₂ := fun e x y hbtw ↦ by simp only [Edgeless.E, mem_empty_iff_false, not_false_eq_true,
+        not_inc₂_of_not_edge_mem] at hbtw}
+
+lemma HasHom.rfl : G₁ ≤⟶ G₁ := ⟨HomSys.id, HomSys.IsHomOn.id⟩
+
+lemma HasHom.trans {G₁ : Graph α β} {G₂ : Graph γ δ} {G₃ : Graph ε ζ} (h₁₂ : G₁ ≤⟶ G₂)
+    (h₂₃ : G₂ ≤⟶ G₃) : G₁ ≤⟶ G₃ := by
+  obtain ⟨f₁₂, hf₁₂⟩ := h₁₂
+  obtain ⟨f₂₃, hf₂₃⟩ := h₂₃
+  exact ⟨f₁₂.comp f₂₃, hf₁₂.comp hf₂₃⟩
+
+def IsCore (G : Graph α β) := ∀ f : HomSys α β α β, f.IsHomOn G G → f.IsIsomOn G G
+
+end Hom
